function method

src/linear/layer1/ADT.dfy
@@ -23,12 +23,31 @@ trait ADT<M> {
     reads this, Repr()
     requires Valid()
 
-  predicate ValidDistinct(adts: seq<ADT>)
+  
+}
+
+predicate ValidDistinctADTs(adts: seq<ADT>)
   reads set r | r in adts :: r
   reads BigUnion(set r | r in adts :: r.Repr())
-{
-  && (forall r | r in adts :: r.Valid())
-  && (forall r, s | r in adts && s in adts && [r, s] <= adts ::
+  {
+    && (forall r | r in adts :: r.Valid())
+    && (forall r, s | r in adts && s in adts && [r, s] <= adts ::
         {r} + r.Repr() !! {s} + s.Repr())
-}
-}
+  }
+predicate ValidDistinctObjs(objects: seq<object>)
+  {
+    forall r, s | r in objects && s in objects && [r, s] <= objects ::
+        {r}  !! {s} 
+  }
+predicate ValidDistinct(adts: seq<ADT>, objs: seq<object>)
+  reads set r | r in adts :: r
+  reads BigUnion(set r | r in adts :: r.Repr())
+  {
+   && (forall r | r in adts :: r.Valid())
+   && (forall r, s | r in adts && s in adts && [r, s] <= adts ::
+         {r} + r.Repr() !! {s} + s.Repr())
+   && (forall r, s | r in objs && s in objs && [r, s] <= objs ::
+         {r} !! {s})
+   && (forall r, s | r in adts && s in objs ::
+         {r} + r.Repr() !! {s})
+  }
